fstar/MLS.TreeSync.KeyPackageRef.fst
@@ -12,4 +12,5 @@ open MLS.Result
 val compute_key_package_ref: #bytes:Type0 -> {|crypto_bytes bytes|} -> key_package_nt bytes -> result (key_package_ref_nt bytes)
 let compute_key_package_ref #bytes #cb kp =
   let kp_bytes: bytes = serialize (key_package_nt bytes) kp in
-  make_keypackage_ref kp_bytes
+  res <-- make_keypackage_ref kp_bytes;
+  return (res <: mls_bytes bytes)
